$(2.1)$
	$$\bar{v} = \frac{\Delta x} {\Delta t}\quad$$
	 ^6c341a

$(2.2a)$
$$ v = \lim_{\Delta t \rightarrow 0} \frac{\Delta x} {\Delta t}$$ ^432453

$(2.2a)$
$$\frac{dx}{dt} = \lim_{\Delta t \rightarrow 0} \frac{\Delta x}{\Delta t}$$

$(2.2b)$
$$v = \frac{dx}{dt}$$ ^260405

$(2.3)$
$$\frac{dx}{dt} = nbt^{n-1}$$ ^9da741

$(2.4)$
$$\bar a = \frac{\Delta v}{\Delta t}$$ ^287a23

$(2.5)$
$$a = \lim_{\Delta t \rightarrow 0}\frac{\Delta v}{\Delta t} = \frac{dv}{dt}$$ ^f6d451

$(2.6)$
$$a = \frac{dv}{dt}=\frac{d}{dt}(\frac{dx}{dt}) = \frac{d^2x}{dt^2}$$ ^7dc47d


$$a = \bar a = \frac{\Delta v}{\Delta t} = \frac{v-v_0}{t-0}$$

$(2.7)$
$$v=v_0 + at$$ ^8ad5cb

$(2.8)$
$$\bar v = \frac{1}{2}(v_0+v)$$
$$\bar v = \frac{\Delta x}{\Delta t} = \frac{x-x_0}{t-0}$$ ^fd6ba3

$(2.9)$
$$x = x_0 + \bar vt = x_0 + \frac{1}{2}(v_0 + v)t$$ ^713ef0

$(2.10)$
$$x = x_0 + v_0t + \frac{1}{2}at^2$$ ^ac4931

$(2.11)$
$$v^2 = v_0^2 + 2a(x-x_0)$$ ^8abcbf


$(2.12)$
$$v(t) = \int a(t)dt$$ ^0019e6

$(2.13)$
$$x(t) = \int v(t)dt$$ ^bb6527

$(3.1)$
$$A=\sqrt{A_x^2 + A_y^2}\;,\quad\tan\theta=\frac{A_y}{A_x}$$ ^0c3e0f

$(3.2)$
$$A_x = A\cos\theta,\quad A_y = A\sin\theta$$ ^51cede

$(3.3)$
$$\bar {\vec v} = \frac{\Delta \vec r}{\Delta t}$$
$(3.4)$
$$\vec v = \lim_{\Delta t \to 0}\frac{\Delta \vec r}{\Delta t} =\frac{d\vec r}{dt}$$

$(3.5)$
$$\bar {\vec a} = \frac{\Delta \vec r} {\Delta t}$$

$(3.6)$
$$\vec a = \lim_{\Delta t \to 0}\frac{\Delta \vec v}{\Delta t} = \frac{d\vec v}{dt}$$

$(3.7)$
$$\vec v = \vec{v^\prime} + \vec V$$

$(3.8)$
$$\vec v = \vec v_0 + \vec at$$

$(3.9)$
$$\vec r = \vec r_0 + \vec v_0t + \frac{1}{2}\vec a t^2$$

$(3.10)$
$$v_x = v_{x0}$$

$(3.11)$
$$v_y = v_{y0}-gt$$

$(3.12)$
$$x = x_0 + v_{x0}t$$

$(3.13)$
$$y = y_0 + v_{y0}t-\frac{1}{2}gt^2$$

$(3.14)$
$$y = x\tan\theta_0 - \frac{g}{2v_0^2\cos^2\theta_0}x^2$$

$(3.15)$
$$x = \frac{v_0^2}{g}\sin2\theta_0$$

$(3.16)$
$$a = \frac{v^2}{r}$$


